\documentclass{ximera}

\input{../../preamble.tex}

\author{Jim Talamo}
\license{Creative Commons 3.0 By-bC}


\outcome{}


\begin{document}
\begin{exercise}

Define a sequence recursively by
\[
a_1 = 1, \quad a_2 = 3, \quad a_3 = 10,
\]
and the rule that $a_n = a_{n-1} - a_{n-3}$.  Compute $a_5$.


\[
a_5 = \answer{6}
\]
\begin{hint}
  First we compute $a_4$.  Substituting $4$ for $n$ in the recursive
  rule $a_n = a_{n-1} - a_{n-3}$, we find
  \begin{align*}
  a_4 &= a_{\answer[given]{3}} - a_{\answer[given]{1}} = \answer{9} \\
  \end{align*}
  
  \begin{question}
  Substituting $5$ for $n$ in the rule $a_n = a_{n-1} - a_{n-3}$, we find
  \[
  a_5 = a_{\answer{4}} - a_{\answer{2}}
  \]
  We just computed $a_4 = 9$; we were given $a_2 = 3$.  Therefore:
  \begin{align*}
    a_5&= \answer[given]{6} 
  \end{align*}
  \end{question}
\end{hint}

\end{exercise}
\end{document}
